WIP

Clap/eDSLState/Convert.lean
@@ -25,10 +25,10 @@ structure Converts' {p : ℕ} {α : Type}
   (exprs : List ExprRef)
   (val : α)
 : Prop where
-  len       : ∀ i, (conversion i).length = exprs.length
+  h_conversion : (conversion val).length = exprs.length
   varSet_wf : ∀ (i : Fin exprs.length), ⦃exprs[i], σ⦄.varSet_wellFormed numAlloc
   expr_wf   : ∀ (i : Fin exprs.length), ⦃exprs[i], σ⦄.wellFormed
-  value_eq  : ∀ (i : Fin exprs.length), [varStore|⦃exprs[i], σ⦄] = .some ((conversion val)[i]'(by grind)) -- from `Converts'.len`
+  value_eq  : ∀ (i : Fin exprs.length), [varStore|⦃exprs[i], σ⦄] = .some ((conversion val)[i])
 
 -- structure HasSpec {p} {idealT} {representsT} (action : ClapM p representsT) where
 --   spec : idealT
